\documentclass[12pt]{article}
\usepackage{amsfonts}
\usepackage[hscale=.8,vscale=.8]{geometry}
\usepackage{hyperref}

\begin{document}

\title{Notes on Feller Condition}
\date{Dec. 32, 2999}

\maketitle

\section{Fokker-Planck Equation}

  Consider the following paraboic partial differential equation (PDE) \cite{Feller}
  \begin{equation}
    \frac{\partial u(t,x)}{\partial t} = -\frac{\partial}{\partial x}\left((bx+c)u(t,x)\right)
                                       + \frac{\partial^2}{\partial x^2}\left(axu(t,x)\right),
    \label{FP}
  \end{equation}
  with $x>0$. This can be viewed as the corresponding Fokker-Planck equation for the Cox-Ingersoll-Ross (CIR)
  process
  \begin{equation}
    dx_t=\kappa(\theta-x_t)dt + \sigma\sqrt{x_t}dW_t,
  \end{equation}
  with $a=\sigma^2/2$, $b=-\kappa$, and $c=\kappa\theta$.

  We want to find the fundamental solution of the PDE (\ref{FP}), {\it i.e.}, the initial condition is given
  by
  \begin{equation}
    u(0,x)=\delta(x-y),
  \end{equation}
  where $\delta(x)$ is the Dirac delta function. To this end, introduce the Laplace transform of $u(t,x)$ as
  \begin{equation}
    v(t,\lambda)=\int_0^{+\infty}e^{-\lambda x}u(t,x)dx,
  \end{equation}
  for $\lambda > 0$. Consider the Laplace transform of the right hand side of Eq. (\ref{FP}),
  \begin{eqnarray}
      && \int_0^{+\infty} e^{-\lambda x}\left[\left(axu(t,x)\right)_{xx}-\left((bx+c)u(t,x)\right)_x\right]dx \nonumber\\
    = && \left. e^{-\lambda x}\left[\left(axu(t,x)\right)_{x}-\left((bx+c)u(t,x)\right)\right]\right|_0^{+\infty}\nonumber\\
      && \quad\quad \lambda \int_0^{+\infty} e^{-\lambda x}\left[\left(axu(t,x)\right)_{x}-\left((bx+c)u(t,x)\right)\right]dx \nonumber\\
    = && f(t) + \lambda(b-\lambda a)v_s - c\lambda v,
  \end{eqnarray}
  where
  \begin{equation}
    f(t) = \lim_{x\rightarrow 0}\left[(bx+c)u-(axu)_x\right],
  \end{equation}
  is the flux at $x=0$ and cannot be arbitrarily specified.

  After the Laplace transform, Eq. (\ref{FP}) becomes
  \begin{equation}
    v_t + \lambda(\lambda a - b) v_s = f(t) - c\lambda v.
  \end{equation}
  This first order PDE can be solved by the method of characteristics.


\begin{thebibliography}{99}
  \bibitem{Feller}
    W. Feller, {\it Two Singular Diffusion Problems}, Annals of Mathematics {\bf 54}, 173 (1951).

\end{thebibliography}


\end{document}